Wire cb_loc: Loc in CyclicBufferTokens and Impl

concurrency/node-replication/Impl.i.dfy
@@ -206,9 +206,9 @@ module Impl(nrifc: NRIfc) {
     linear localTail: Atomic<uint64, LocalTailTokens>
   )
   {
-    predicate WF(nodeId: nat) {
+    predicate WF(nodeId: nat, cb_loc: Loc) {
       && (forall v, g :: atomic_inv(localTail, v, g) <==>
-          g == LocalTailTokens(LocalTail(nodeId, v as int), CBLocalTail(nodeId, v as int)))
+          g == LocalTailTokens(LocalTail(nodeId, v as int), CBLocalTail(nodeId, v as int, cb_loc)))
     }
   }
 
@@ -216,14 +216,14 @@ module Impl(nrifc: NRIfc) {
     linear cell: Cell<CB.ConcreteLogEntry>,
     linear alive: Atomic<bool, CBAliveBit>)
   {
-    predicate WF(i: nat)
+    predicate WF(i: nat, cb_loc: Loc)
     {
-      && (forall v, g :: atomic_inv(alive, v, g) <==> g == CBAliveBit(i, v))
+      && (forall v, g :: atomic_inv(alive, v, g) <==> g == CBAliveBit(i, v, cb_loc))
       && alive.namespace() == 0
     }
   }
 
-  predicate BufferEntryInv(buffer: lseq<BufferEntry>, i: int, t: CB.StoredType)
+  predicate BufferEntryInv(buffer: lseq<BufferEntry>, i: int, t: CB.StoredType, cb_loc: Loc)
   requires |buffer| == LOG_SIZE as int
   {
     && t.cellContents.cell == buffer[i % LOG_SIZE as int].cell
@@ -235,10 +235,10 @@ module Impl(nrifc: NRIfc) {
     )
   }
 
-  predicate ContentsInv(buffer: lseq<BufferEntry>, contents: CBContents)
+  predicate ContentsInv(buffer: lseq<BufferEntry>, contents: CBContents, cb_loc: Loc)
   requires |buffer| == LOG_SIZE as int
   {
-    && (forall i | i in contents.contents :: BufferEntryInv(buffer, i, contents.contents[i]))
+    && (forall i | i in contents.contents :: BufferEntryInv(buffer, i, contents.contents[i], cb_loc))
   }
 
   linear datatype NR = NR(
@@ -248,21 +248,23 @@ module Impl(nrifc: NRIfc) {
     linear node_info: lseq<NodeInfo>, // NodeInfo is padded
 
     linear buffer: lseq<BufferEntry>,
-    glinear bufferContents: GhostAtomic<CBContents>
+    glinear bufferContents: GhostAtomic<CBContents>,
+
+    ghost cb_loc: Loc
   )
   {
     predicate WF() {
       && (forall v, g :: atomic_inv(ctail.inner, v, g) <==> g == Ctail(v as int))
-      && (forall v, g :: atomic_inv(head.inner, v, g) <==> g == CBHead(v as int))
+      && (forall v, g :: atomic_inv(head.inner, v, g) <==> g == CBHead(v as int, cb_loc))
       && (forall v, g :: atomic_inv(globalTail.inner, v, g) <==>
-            g == GlobalTailTokens(GlobalTail(v as int), CBGlobalTail(v as int)))
+            g == GlobalTailTokens(GlobalTail(v as int), CBGlobalTail(v as int, cb_loc)))
       && |node_info| == NUM_REPLICAS as int
       && (forall nodeId | 0 <= nodeId < |node_info| :: nodeId in node_info)
-      && (forall nodeId | 0 <= nodeId < |node_info| :: node_info[nodeId].WF(nodeId))
+      && (forall nodeId | 0 <= nodeId < |node_info| :: node_info[nodeId].WF(nodeId, cb_loc))
       && |buffer| == LOG_SIZE as int
-      && (forall v, g :: atomic_inv(bufferContents, v, g) <==> ContentsInv(buffer, g))
+      && (forall v, g :: atomic_inv(bufferContents, v, g) <==> ContentsInv(buffer, g, cb_loc))
       && (forall i: nat | 0 <= i < LOG_SIZE as int :: i in buffer)
-      && (forall i: nat | 0 <= i < LOG_SIZE as int :: buffer[i].WF(i))
+      && (forall i: nat | 0 <= i < LOG_SIZE as int :: buffer[i].WF(i, cb_loc))
 
       && bufferContents.namespace() == 1
       && globalTail.inner.namespace() == 0
@@ -972,6 +974,7 @@ module Impl(nrifc: NRIfc) {
     glinear cb': CBCombinerToken)
   requires nr.WF()
   requires node.WF()
+  requires nr.cb_loc == cb.cb_loc
   requires |ops| == MAX_THREADS_PER_REPLICA as int
   requires |requestIds| == num_ops as int <= MAX_THREADS_PER_REPLICA as int
   requires combinerState.nodeId == node.nodeId as int
@@ -1014,6 +1017,7 @@ module Impl(nrifc: NRIfc) {
     // invariant cb' == cb
     invariant cb'.nodeId == cb.nodeId
     invariant cb'.rs.CombinerIdle?
+    invariant cb'.cb_loc == cb.cb_loc
     invariant ghost_replica'.state == nrifc.I(actual_replica')
     invariant ghost_replica'.nodeId == node.nodeId as int
     invariant !done ==>
@@ -1094,7 +1098,7 @@ module Impl(nrifc: NRIfc) {
             }
 
             forall i | i in contents.contents
-            ensures BufferEntryInv(nr.buffer, i, contents.contents[i])
+            ensures BufferEntryInv(nr.buffer, i, contents.contents[i], contents.cb_loc)
             {
             }
 
@@ -1113,6 +1117,7 @@ module Impl(nrifc: NRIfc) {
           invariant cb'.rs.CombinerAppending?
           invariant cb'.rs.cur_idx == tail as int + j as int
           invariant cb'.rs.tail == tail as int + num_ops as int
+          invariant cb'.cb_loc == cb.cb_loc
           invariant forall i: int | j as int <= i < |requestIds| ::
               i in log_entries
                 && log_entries[i] == Log(tail as int + i, ops[i], node.nodeId as int)
@@ -1129,7 +1134,7 @@ module Impl(nrifc: NRIfc) {
                 glmap_take(cyclic_buffer_entries, tail as int + j as int);
 
             assert BufferEntryInv(nr.buffer,
-                (tail as int + j as int) - LOG_SIZE as int, cyclic_buffer_entry);
+                (tail as int + j as int) - LOG_SIZE as int, cyclic_buffer_entry, cb'.cb_loc);
 
             glinear var StoredType(cellContents, oldLogEntry) := cyclic_buffer_entry;
 
@@ -1141,7 +1146,7 @@ module Impl(nrifc: NRIfc) {
               bounded_idx as int;
             }
 
-            assert nr.buffer[bounded_idx as int].WF(bounded_idx as int);
+            assert nr.buffer[bounded_idx as int].WF(bounded_idx as int, cb'.cb_loc);
 
             // Physically write the log entry into the cyclic buffer
             write_cell(lseq_peek(nr.buffer, bounded_idx).cell,
@@ -1150,7 +1155,7 @@ module Impl(nrifc: NRIfc) {
             
             cyclic_buffer_entry := CB.StoredType(cellContents, glSome(log_entry));
             assert BufferEntryInv(nr.buffer,
-                (tail as int + j as int), cyclic_buffer_entry);
+                (tail as int + j as int), cyclic_buffer_entry, cb'.cb_loc);
 
             var m := ((tail + j) / LOG_SIZE) % 2 == 0;
             atomic_block var _ := execute_atomic_store(
@@ -1279,7 +1284,7 @@ module Impl(nrifc: NRIfc) {
     cb' := cb;
     responses' := responses;
 
-    assert nr.node_info[node.nodeId as int].WF(node.nodeId as int);
+    assert nr.node_info[node.nodeId as int].WF(node.nodeId as int, cb'.cb_loc);
 
     ghost var requestIds' := requestIds;
     if combinerState'.state.CombinerReady? {
@@ -1326,7 +1331,7 @@ module Impl(nrifc: NRIfc) {
       invariant combinerState'.state.Combiner?
       invariant combinerState'.state.queueIndex == responsesIndex as int
       invariant combinerState'.state == prev_combinerState.state.(localTail := i as int).(queueIndex := responsesIndex as int)
-      invariant cb' == CBCombinerToken(node.nodeId as int, CB.CombinerReading(CB.ReaderRange(ltail as int, gtail as int, i as nat)))
+      invariant cb' == CBCombinerToken(node.nodeId as int, CB.CombinerReading(CB.ReaderRange(ltail as int, gtail as int, i as nat)), cb.cb_loc)
       invariant ghost_replica'.state == nrifc.I(actual_replica')
       invariant ghost_replica'.nodeId == node.nodeId as int
       invariant |responses'| == MAX_THREADS_PER_REPLICA as int
@@ -1348,7 +1353,7 @@ module Impl(nrifc: NRIfc) {
         var done := false;
         while !done
         invariant 0 <= iteration as int <= WARN_THRESHOLD as int
-        invariant cb' == CBCombinerToken(node.nodeId as int, CB.CombinerReading(CB.ReaderRange(ltail as int, gtail as int, if !done then i as nat else i as nat + 1)))
+        invariant cb' == CBCombinerToken(node.nodeId as int, CB.CombinerReading(CB.ReaderRange(ltail as int, gtail as int, if !done then i as nat else i as nat + 1)), cb.cb_loc)
         invariant ghost_replica'.state == nrifc.I(actual_replica')
         invariant ghost_replica'.nodeId == node.nodeId as int
         invariant combinerState'.nodeId == prev_combinerState.nodeId
