concurrency/node-replication/Init.i.dfy
@@ -31,14 +31,15 @@ module Init(nrifc: NRIfc) {
     nodeId: uint64,
     glinear combiner: CombinerToken,
     glinear cb: CBCombinerToken,
-    glinear ghost_replica: Replica)
+    glinear ghost_replica: Replica,
+    ghost cb_loc: Loc)
   {
     predicate WF()
     {
       && 0 <= nodeId as int < NUM_REPLICAS as int
       && ghost_replica == Replica(nodeId as int, nrifc.init_state())
       && combiner == CombinerToken(nodeId as int, CombinerReady)
-      && cb == CBCombinerToken(nodeId as int, CB.CombinerIdle)
+      && cb == CBCombinerToken(nodeId as int, CB.CombinerIdle, cb_loc)
     }
   }
 
@@ -50,7 +51,7 @@ module Init(nrifc: NRIfc) {
   ensures forall i | 0 <= i < |owned_contexts| ::
     i in owned_contexts && owned_contexts[i].WF(node)
   {
-    linear var NodeCreationToken(nodeId, combiner, cb, ghost_replica) := nct;
+    linear var NodeCreationToken(nodeId, combiner, cb, ghost_replica, cb_loc) := nct;
 
     // initialize the flat_combiner ghost tokens
 
@@ -215,14 +216,14 @@ module Init(nrifc: NRIfc) {
       glinear alive: map<nat, CBAliveBit>)
   returns (linear buffer: lseq<BufferEntry>)
   requires |cells| == LOG_SIZE as int
-  requires forall i | 0 <= i < LOG_SIZE as int ::
+  requires exists cb_loc :: forall i | 0 <= i < LOG_SIZE as int ::
       && i in cells
       && i in alive
-      && alive[i] == CBAliveBit(i, false)
+      && alive[i] == CBAliveBit(i, false, cb_loc)
   ensures |buffer| == LOG_SIZE as int
   ensures forall i | 0 <= i < LOG_SIZE as int
     :: i in buffer && buffer[i].cell == cells[i]
-        && buffer[i].WF(i)
+        && buffer[i].WF(i, alive[i].cb_loc)
   {
     buffer := lseq_alloc(LOG_SIZE);
     linear var cells' := cells;
@@ -234,7 +235,7 @@ module Init(nrifc: NRIfc) {
     invariant |buffer| == LOG_SIZE as int
     invariant forall i | 0 <= i < j as int
       :: i in buffer && buffer[i].cell == cells[i]
-          && buffer[i].WF(i)
+          && buffer[i].WF(i, alive[i].cb_loc)
     invariant forall i | j as int <= i < LOG_SIZE as int
       :: i !in buffer
     invariant |cells'| == LOG_SIZE as int
@@ -254,11 +255,11 @@ module Init(nrifc: NRIfc) {
       alive', aliveBit := glmap_take(alive', j as int);
 
       linear var aliveAtomic := new_atomic(false, aliveBit,
-          ((v, g) => g == CBAliveBit(j as int, v)),
+          ((v, g) => g == CBAliveBit(j as int, v, alive[j as nat].cb_loc)),
           0);
 
       linear var bufferEntry := BufferEntry(cell, aliveAtomic);
-      assert bufferEntry.WF(j as int);
+      assert bufferEntry.WF(j as int, alive[j as nat].cb_loc);
 
       buffer := lseq_give(buffer, j, bufferEntry);
 
@@ -278,14 +279,14 @@ module Init(nrifc: NRIfc) {
       glinear localTails: map<nat, LocalTail>,
       glinear cbLocalTails: map<nat, CBLocalTail>)
   returns (linear node_info: lseq<NodeInfo>)
-  requires forall i | 0 <= i < NUM_REPLICAS as int ::
+  requires exists cb_loc :: forall i | 0 <= i < NUM_REPLICAS as int ::
       && i in localTails
       && i in cbLocalTails
       && localTails[i] == LocalTail(i as int, 0)
-      && cbLocalTails[i] == CBLocalTail(i as int, 0)
+      && cbLocalTails[i] == CBLocalTail(i as int, 0, cb_loc)
   ensures |node_info| == NUM_REPLICAS as int
   ensures forall i | 0 <= i < NUM_REPLICAS as int
-      :: i in node_info && node_info[i].WF(i)
+      :: i in node_info && node_info[i].WF(i, cbLocalTails[i].cb_loc)
   {
     node_info := lseq_alloc(NUM_REPLICAS);
 
@@ -299,10 +300,10 @@ module Init(nrifc: NRIfc) {
         && i in localTails'
         && i in cbLocalTails'
         && localTails'[i] == LocalTail(i as int, 0)
-        && cbLocalTails'[i] == CBLocalTail(i as int, 0)
+        && cbLocalTails'[i] == CBLocalTail(i as int, 0, cbLocalTails[i].cb_loc)
     invariant |node_info| == NUM_REPLICAS as int
     invariant forall i | 0 <= i < j as int
-        :: i in node_info && node_info[i].WF(i)
+        :: i in node_info && node_info[i].WF(i, cbLocalTails[i].cb_loc)
     invariant forall i | j as int <= i < NUM_REPLICAS as int
         :: i !in node_info
     {
@@ -314,12 +315,12 @@ module Init(nrifc: NRIfc) {
           0,
           LocalTailTokens(localTail, cbLocalTail),
           ((v, g) => 
-            g == LocalTailTokens(LocalTail(j as int, v as int), CBLocalTail(j as int, v as int))
+            g == LocalTailTokens(LocalTail(j as int, v as int), CBLocalTail(j as int, v as int, cbLocalTails[j as nat].cb_loc))
           ),
           0);
 
       linear var nodeInfo := NodeInfo(localTailAtomic);
-      assert nodeInfo.WF(j as int);
+      assert nodeInfo.WF(j as int, cbLocalTails[j as nat].cb_loc);
 
       node_info := lseq_give(node_info, j, nodeInfo);
 
@@ -335,13 +336,13 @@ module Init(nrifc: NRIfc) {
       glinear combiners: map<nat, CombinerToken>,
       glinear readers: map<nat, CBCombinerToken>)
   returns (linear nodeCreationTokens: lseq<NodeCreationToken>)
-  requires forall i | 0 <= i < NUM_REPLICAS as int ::
+  requires exists cb_loc :: forall i | 0 <= i < NUM_REPLICAS as int ::
       && i in replicas
       && i in combiners
       && i in readers
       && replicas[i] == Replica(i, nrifc.init_state())
       && combiners[i] == CombinerToken(i, CombinerReady)
-      && readers[i] == CBCombinerToken(i, CB.CombinerIdle)
+      && readers[i] == CBCombinerToken(i, CB.CombinerIdle, cb_loc)
   ensures |nodeCreationTokens| == NUM_REPLICAS as int
   ensures forall i | 0 <= i < NUM_REPLICAS as int
       :: i in nodeCreationTokens && nodeCreationTokens[i].WF()
@@ -373,7 +374,7 @@ module Init(nrifc: NRIfc) {
       combiners', combiner := glmap_take(combiners', j as int);
       readers', cb := glmap_take(readers', j as int);
 
-      linear var nct := NodeCreationToken(j, combiner, cb, replica);
+      linear var nct := NodeCreationToken(j, combiner, cb, replica, readers[j as nat].cb_loc);
       assert nct.WF();
 
       nodeCreationTokens := lseq_give(nodeCreationTokens, j, nct);
@@ -403,7 +404,7 @@ module Init(nrifc: NRIfc) {
     buffer_cells, buffer_cell_contents := make_buffer_cells();
 
     glinear var globalTail, replicas, localTails, ctail, combiners := perform_Init(token);
-    glinear var cbHead, cbGlobalTail, cbLocalTails, alive, cbContents, readers :=
+    glinear var cbHead, cbGlobalTail, cbLocalTails, alive, cbContents, readers, cb_loc :=
         cyclic_buffer_init(buffer_cell_contents);
 
     linear var ctail_atomic: Atomic<uint64, Ctail> := new_atomic(
@@ -414,24 +415,24 @@ module Init(nrifc: NRIfc) {
     linear var head_atomic: Atomic<uint64, CBHead> := new_atomic(
         0,
         cbHead,
-        (v, g) => g == CBHead(v as int),
+        (v, g) => g == CBHead(v as int, cb_loc),
         0);
     linear var globalTail_atomic: Atomic<uint64, GlobalTailTokens> := new_atomic(
           0,
           GlobalTailTokens(globalTail, cbGlobalTail),
-          ((v, g) => g == GlobalTailTokens(GlobalTail(v as int), CBGlobalTail(v as int))),
+          ((v, g) => g == GlobalTailTokens(GlobalTail(v as int), CBGlobalTail(v as int, cb_loc))),
           0);
 
     linear var buffer: lseq<BufferEntry> := make_buffer(buffer_cells, alive);
 
     glinear var bufferContents: GhostAtomic<CBContents> := new_ghost_atomic(
         cbContents,
-        (g) => ContentsInv(buffer, g),
+        (g) => ContentsInv(buffer, g, cb_loc),
         1);
 
     linear var node_infos: lseq<NodeInfo> := make_node_infos(localTails, cbLocalTails);
 
-    nr := NR(CachePadded(ctail_atomic), CachePadded(head_atomic), CachePadded(globalTail_atomic), node_infos, buffer, bufferContents);
+    nr := NR(CachePadded(ctail_atomic), CachePadded(head_atomic), CachePadded(globalTail_atomic), node_infos, buffer, bufferContents, cb_loc);
 
     nodeCreationTokens := make_node_creation_tokens(replicas, combiners, readers);
   }
